work on Imp.v without the last one

lf/Imp.v
@@ -463,13 +463,23 @@ Admitted.
     it is sound.  Use the tacticals we've just seen to make the proof
     as short and elegant as possible. *)
 
-Fixpoint optimize_0plus_b (b : bexp) : bexp
-  (* REPLACE THIS LINE WITH ":= _your_definition_ ." *). Admitted.
+Fixpoint optimize_0plus_b (b : bexp) : bexp :=
+  match b with
+  | BTrue => BTrue
+  | BFalse => BFalse
+  | BEq a1 a2 => BEq (optimize_0plus a1) (optimize_0plus a2)
+  | BNeq a1 a2 => BNeq (optimize_0plus a1) (optimize_0plus a2)
+  | BLe a1 a2 => BLe (optimize_0plus a1) (optimize_0plus a2)
+  | BGt a1 a2 => BGt (optimize_0plus a1) (optimize_0plus a2)
+  | other => other
+  end.
 
 Theorem optimize_0plus_b_sound : forall b,
   beval (optimize_0plus_b b) = beval b.
 Proof.
-  (* FILL IN HERE *) Admitted.
+  intros. destruct b;
+  try (simpl; repeat (rewrite optimize_0plus_sound); reflexivity).
+Qed.
 (** [] *)
 
 (** **** Exercise: 4 stars, standard, optional (optimize)
@@ -847,14 +857,34 @@ Qed.
 
 Reserved Notation "e '==>b' b" (at level 90, left associativity).
 Inductive bevalR: bexp -> bool -> Prop :=
-(* FILL IN HERE *)
+  | E_BTrue : BTrue ==>b true
+  | E_BFalse : BFalse ==>b false
+  | E_Beq (a1 a2: aexp) (n1 n2: nat) : a1 ==> n1 -> a2 ==> n2 -> BEq a1 a2 ==>b n1 =? n2
+  | E_BNeq (a1 a2: aexp) (n1 n2 : nat) : a1 ==> n1 -> a2 ==> n2 -> BNeq a1 a2 ==>b negb (n1 =? n2)
+  | E_Ble (a1 a2: aexp) (n1 n2 : nat) : a1 ==> n1 -> a2 ==> n2 -> BLe a1 a2 ==>b n1 <=? n2
+  | E_BGt (a1 a2: aexp) (n1 n2 : nat) : a1 ==> n1 -> a2 ==> n2 -> BGt a1 a2 ==>b negb (n1 <=? n2)
+  | E_BNot (b: bexp) (bv: bool) : b ==>b bv -> BNot b ==>b negb bv
+  | E_BAnd (b1 b2: bexp) (bv1 bv2: bool) : b1 ==>b bv1 -> b2 ==>b bv2 -> BAnd b1 b2 ==>b andb bv1 bv2
 where "e '==>b' b" := (bevalR e b) : type_scope
 .
 
 Lemma beval_iff_bevalR : forall b bv,
   b ==>b bv <-> beval b = bv.
 Proof.
-  (* FILL IN HERE *) Admitted.
+  intros.
+  split.
+  - intros H. induction H; simpl; try reflexivity;
+    try rewrite aeval_iff_aevalR in H;
+	try rewrite aeval_iff_aevalR in H0;
+	try (subst; constructor).
+  - intros H. destruct b; subst; constructor;
+    try (apply aeval_iff_aevalR; reflexivity);
+	[ | rename b1 into b | rename b2 into b]; 
+	induction b; constructor;
+	try (apply aeval_iff_aevalR; reflexivity);
+	try (apply IHb); try (apply IHb1); try (apply IHb2).
+Qed.
+
 (** [] *)
 
 End AExp.
@@ -1542,7 +1572,12 @@ Example ceval_example2:
     Z := 2
   ]=> (Z !-> 2 ; Y !-> 1 ; X !-> 0).
 Proof.
-  (* FILL IN HERE *) Admitted.
+  apply E_Seq with (X !-> 0).
+  - apply E_Asgn. reflexivity.
+  - apply E_Seq with (Y !-> 1; X !-> 0).
+	+ apply E_Asgn. reflexivity.
+	+ apply E_Asgn. reflexivity.
+Qed.
 (** [] *)
 
 Set Printing Implicit.
@@ -1556,16 +1591,32 @@ Check @ceval_example2.
     which you can reverse-engineer to discover the program you should
     write.  The proof of that theorem will be somewhat lengthy. *)
 
-Definition pup_to_n : com
-  (* REPLACE THIS LINE WITH ":= _your_definition_ ." *). Admitted.
+Definition pup_to_n : com := 
+  <{ Y := 0;
+     while (X > 0) do 
+	   Y := Y + X;
+	   X := X - 1
+	 end}>.
 
 Theorem pup_to_2_ceval :
   (X !-> 2) =[
     pup_to_n
   ]=> (X !-> 0 ; Y !-> 3 ; X !-> 1 ; Y !-> 2 ; Y !-> 0 ; X !-> 2).
 Proof.
-  (* FILL IN HERE *) Admitted.
-(** [] *)
+  apply E_Seq with (Y !-> 0; X !-> 2).
+  - apply E_Asgn. reflexivity.
+  - apply E_WhileTrue with (X !-> 1; Y !-> 2; Y !-> 0; X !-> 2).
+    + reflexivity.
+	+ apply E_Seq with (Y !-> 2; Y !-> 0; X !-> 2).
+	  * apply E_Asgn. reflexivity.
+	  * apply E_Asgn. reflexivity.
+	+ apply E_WhileTrue with (X !-> 0; Y !-> 3; X !-> 1; Y !-> 2; Y !-> 0; X !-> 2).
+	  * reflexivity.
+	  * apply E_Seq with (Y !-> 3; X !-> 1; Y !-> 2; Y !-> 0; X !-> 2).
+	    ** apply E_Asgn. reflexivity.
+		** apply E_Asgn. reflexivity.
+	  * apply E_WhileFalse. reflexivity.
+Qed.
 
 (* ================================================================= *)
 (** ** Determinism of Evaluation *)
@@ -1640,11 +1691,24 @@ Proof.
 
     State and prove a specification of [XtimesYinZ]. *)
 
+Print XtimesYinZ.
+
 (* FILL IN HERE *)
+
+Theorem XtimesYinZ_spec : forall st n1 n2 st',
+  st X = n1 ->
+  st Y = n2 ->
+  st =[ XtimesYinZ ]=> st' ->
+  st' Z = n1 * n2.
+Proof.
+  intros. inversion H1. subst. simpl. apply t_update_eq.  
+Qed.
 
 (* Do not modify the following line: *)
 Definition manual_grade_for_XtimesYinZ_spec : option (nat*string) := None.
 (** [] *)
+
+Print loop.
 
 (** **** Exercise: 3 stars, standard, especially useful (loop_never_stops) *)
 Theorem loop_never_stops : forall st st',
@@ -1659,7 +1723,11 @@ Proof.
       contradictory and so can be solved in one step with
       [discriminate]. *)
 
-  (* FILL IN HERE *) Admitted.
+  induction contra; try discriminate.
+  - injection Heqloopdef as H0 H1. 
+    rewrite H0 in H. simpl in H. inversion H.
+  - apply IHcontra2. apply Heqloopdef.
+Qed.
 (** [] *)
 
 (** **** Exercise: 3 stars, standard (no_whiles_eqv)
@@ -1686,13 +1754,32 @@ Fixpoint no_whiles (c : com) : bool :=
     while loops.  Then prove its equivalence with [no_whiles]. *)
 
 Inductive no_whilesR: com -> Prop :=
- (* FILL IN HERE *)
+  | no_whilesR_Skip: no_whilesR <{ skip }>
+  | no_whilesR_Asgn : forall x a, no_whilesR <{ x := a }>
+  | no_whilesR_Seq : forall c1 c2, 
+    no_whilesR c1 -> no_whilesR c2 -> no_whilesR <{ c1 ; c2 }>
+  | no_whilesR_If : forall b c1 c2,
+    no_whilesR c1 -> no_whilesR c2 -> no_whilesR <{ if b then c1 else c2 end }>
 .
 
 Theorem no_whiles_eqv:
   forall c, no_whiles c = true <-> no_whilesR c.
 Proof.
-  (* FILL IN HERE *) Admitted.
+  split.
+  - intros. induction c.
+    + apply no_whilesR_Skip.
+	+ apply no_whilesR_Asgn.
+	+ simpl in H. rewrite andb_true_iff in H.
+	  destruct H as [H1 H2]. apply IHc1 in H1. apply IHc2 in H2.
+	  constructor.  apply H1. apply H2.
+	+ simpl in H. rewrite andb_true_iff in H.
+	  destruct H as [H1 H2]. apply IHc1 in H1. apply IHc2 in H2.
+	  constructor. apply H1. apply H2.
+	+ simpl in H. discriminate.
+  - intros H. induction H; simpl; try reflexivity; 
+    apply andb_true_iff; split; try apply IHno_whilesR1; try apply IHno_whilesR2.
+Qed.
+    
 (** [] *)
 
 (** **** Exercise: 4 stars, standard (no_whiles_terminating)
@@ -1702,6 +1789,22 @@ Proof.
 
     Use either [no_whiles] or [no_whilesR], as you prefer. *)
 
+Theorem no_whiles_terminating : forall st c,
+  no_whilesR c -> exists st', st =[ c ]=> st'.
+Proof.
+  intros. generalize dependent st. induction H; intros st.
+  - exists st. apply E_Skip.
+  - exists (x !-> aeval st a; st). apply E_Asgn. reflexivity.
+  - destruct (IHno_whilesR1 st) as [st1 H1].
+    destruct (IHno_whilesR2 st1) as [st2 H2].
+	exists st2. apply E_Seq with st1. apply H1. apply H2.
+  - destruct (IHno_whilesR1 st) as [st1 H1].
+	destruct (IHno_whilesR2 st) as [st2 H2].
+	destruct (beval st b) eqn:Eqb.
+	+ exists st1. apply E_IfTrue. apply Eqb. apply H1.
+	+ exists st2. apply E_IfFalse. apply Eqb. apply H2.
+Qed.
+	
 (* FILL IN HERE *)
 
 (* Do not modify the following line: *)
@@ -1773,8 +1876,16 @@ Inductive sinstr : Type :=
 
 Fixpoint s_execute (st : state) (stack : list nat)
                    (prog : list sinstr)
-                 : list nat
-  (* REPLACE THIS LINE WITH ":= _your_definition_ ." *). Admitted.
+                 : list nat :=
+  match prog, stack with
+  | [], _ => stack
+  | SPush n :: prog', _ => s_execute st (n :: stack) prog'
+  | SLoad v :: prog',_ => s_execute st (st v :: stack) prog'
+  | SPlus :: prog', x :: y :: stack' => s_execute st ((x + y) :: stack') prog'
+  | SMinus :: prog', x :: y :: stack' => s_execute st ((y - x) :: stack') prog'
+  | SMult :: prog', x :: y :: stack' => s_execute st ((x * y) :: stack') prog'
+  | _ :: prog', _ => s_execute st stack prog'
+  end.
 
 Check s_execute.
 
@@ -1782,20 +1893,26 @@ Example s_execute1 :
      s_execute empty_st []
        [SPush 5; SPush 3; SPush 1; SMinus]
    = [2; 5].
-(* FILL IN HERE *) Admitted.
+Proof. reflexivity. Qed.
 
 Example s_execute2 :
      s_execute (X !-> 3) [3;4]
        [SPush 4; SLoad X; SMult; SPlus]
    = [15; 4].
-(* FILL IN HERE *) Admitted.
+Proof. reflexivity. Qed.
 
 (** Next, write a function that compiles an [aexp] into a stack
     machine program. The effect of running the program should be the
     same as pushing the value of the expression on the stack. *)
 
-Fixpoint s_compile (e : aexp) : list sinstr
-  (* REPLACE THIS LINE WITH ":= _your_definition_ ." *). Admitted.
+Fixpoint s_compile (e : aexp) : list sinstr :=
+  match e with
+  | ANum n => [SPush n]
+  | AId v => [SLoad v]
+  | APlus a1 a2 => s_compile a1 ++ s_compile a2 ++ [SPlus]
+  | AMinus a1 a2 => s_compile a1 ++ s_compile a2 ++ [SMinus]
+  | AMult a1 a2 => s_compile a1 ++ s_compile a2 ++ [SMult]
+  end.
 
 (** After you've defined [s_compile], prove the following to test
     that it works. *)
@@ -1803,7 +1920,7 @@ Fixpoint s_compile (e : aexp) : list sinstr
 Example s_compile1 :
   s_compile <{ X - (2 * Y) }>
   = [SLoad X; SPush 2; SLoad Y; SMult; SMinus].
-(* FILL IN HERE *) Admitted.
+Proof. reflexivity. Qed.
 (** [] *)
 
 (** **** Exercise: 3 stars, standard (execute_app) *)
@@ -1816,8 +1933,12 @@ Example s_compile1 :
 Theorem execute_app : forall st p1 p2 stack,
   s_execute st stack (p1 ++ p2) = s_execute st (s_execute st stack p1) p2.
 Proof.
-  (* FILL IN HERE *) Admitted.
-
+  intros st p1. induction p1.
+  - simpl. reflexivity.
+  - intros. destruct stack.
+    + destruct a; simpl; apply IHp1.
+	+ destruct a; destruct stack; simpl; apply IHp1.
+Qed.
 (** [] *)
 
 (** **** Exercise: 3 stars, standard (stack_compiler_correct) *)
@@ -1830,14 +1951,21 @@ Proof.
 Lemma s_compile_correct_aux : forall st e stack,
   s_execute st stack (s_compile e) = aeval st e :: stack.
 Proof.
-  (* FILL IN HERE *) Admitted.
+  intros st e. induction e; simpl; try reflexivity; intros stack;
+  rewrite execute_app; rewrite IHe1;
+  rewrite execute_app; rewrite IHe2; simpl. 
+  - rewrite (add_comm (aeval st e1) (aeval st e2)). reflexivity.
+  - reflexivity.
+  - rewrite (mul_comm (aeval st e1) (aeval st e2)). reflexivity.
+Qed.
 
 (** The main theorem should be a very easy corollary of that lemma. *)
 
 Theorem s_compile_correct : forall (st : state) (e : aexp),
   s_execute st [] (s_compile e) = [ aeval st e ].
 Proof.
-  (* FILL IN HERE *) Admitted.
+  intros. apply s_compile_correct_aux.
+Qed.
 
 (** [] *)
 
@@ -1859,8 +1987,25 @@ Proof.
     programs terminate.) *)
 
 (* FILL IN HERE
-
     [] *)
+
+Fixpoint beval_sc (st : state) (b : bexp) : bool :=
+  match b with 
+  | <{ true }> => true
+  | <{ false }> => false
+  | <{ a1 = a2 }> => aeval st a1 =? aeval st a2
+  | <{ a1 <> a2 }> => negb (aeval st a1 =? aeval st a2)
+  | <{ a1 <= a2 }> => aeval st a1 <=? aeval st a2
+  | <{ a1 > a2 }> => negb (aeval st a1 <=? aeval st a2)
+  | <{ ~b }> => negb (beval_sc st b)
+  | <{ b1 && b2 }> => if beval_sc st b1 then beval_sc st b2 else false
+  end.
+
+Theorem beval_sc_correct : forall st b,
+  beval st b = beval_sc st b.
+Proof.
+  intros. induction b; simpl; try reflexivity.
+Qed.
 
 Module BreakImp.
 (** **** Exercise: 4 stars, advanced (break_imp)
@@ -1982,8 +2127,38 @@ Reserved Notation "st '=[' c ']=>' st' '/' s"
 Inductive ceval : com -> state -> result -> state -> Prop :=
   | E_Skip : forall st,
       st =[ CSkip ]=> st / SContinue
-  (* FILL IN HERE *)
-
+  | E_Break : forall st,
+      st =[ CBreak ]=> st / SBreak
+  | E_Asgn : forall st a n x,
+      aeval st a = n ->
+	  	st =[ x := a ]=> (x !-> n; st) / SContinue
+  | E_Seq1 : forall st c1 c2 st' st'' r,
+			st =[ c1 ]=> st' / SContinue ->
+			st' =[ c2 ]=> st'' / r ->
+			st =[ c1 ; c2 ]=> st'' / r
+	| E_Seq2 : forall st c1 c2 st',
+	 		st =[ c1 ]=> st' / SBreak ->
+			st =[ c1 ; c2 ]=> st' / SBreak
+	| E_IfTrue : forall st b c1 c2 st' r,
+			beval st b = true ->
+			st =[ c1 ]=> st' / r ->
+			st =[ if b then c1 else c2 end ]=> st' / r
+	| E_IfFalse : forall st b c1 c2 st' r,
+			beval st b = false ->
+			st =[ c2 ]=> st' / r ->
+			st =[ if b then c1 else c2 end ]=> st' / r
+	| E_WhileTrue : forall st b c st' st'' r,
+			beval st b = true ->
+			st =[ c ]=> st' / SContinue ->
+			st' =[ while b do c end ]=> st'' / r ->
+			st =[ while b do c end ]=> st'' / SContinue
+	| E_WhileFalse : forall st b c,
+			beval st b = false ->
+			st =[ while b do c end ]=> st / SContinue
+	| E_WhileBreak : forall st b c st',
+			beval st b = true ->
+			st =[ c ]=> st' / SBreak ->
+			st =[ while b do c end ]=> st' / SContinue
   where "st '=[' c ']=>' st' '/' s" := (ceval c st s st').
 
 (** Now prove the following properties of your definition of [ceval]: *)
@@ -1992,33 +2167,40 @@ Theorem break_ignore : forall c st st' s,
      st =[ break; c ]=> st' / s ->
      st = st'.
 Proof.
-  (* FILL IN HERE *) Admitted.
+  intros. inversion H; subst.
+	- inversion H2.
+	- inversion H5. reflexivity.
+Qed.
 
 Theorem while_continue : forall b c st st' s,
   st =[ while b do c end ]=> st' / s ->
   s = SContinue.
 Proof.
-  (* FILL IN HERE *) Admitted.
+  intros. inversion H; reflexivity.
+Qed.
 
 Theorem while_stops_on_break : forall b c st st',
   beval st b = true ->
   st =[ c ]=> st' / SBreak ->
   st =[ while b do c end ]=> st' / SContinue.
 Proof.
-  (* FILL IN HERE *) Admitted.
+  intros. apply E_WhileBreak; assumption.
+Qed.
 
 Theorem seq_continue : forall c1 c2 st st' st'',
   st =[ c1 ]=> st' / SContinue ->
   st' =[ c2 ]=> st'' / SContinue ->
   st =[ c1 ; c2 ]=> st'' / SContinue.
 Proof.
-  (* FILL IN HERE *) Admitted.
+  intros. apply E_Seq1 with st'; assumption.
+Qed.
 
 Theorem seq_stops_on_break : forall c1 c2 st st',
   st =[ c1 ]=> st' / SBreak ->
   st =[ c1 ; c2 ]=> st' / SBreak.
 Proof.
-  (* FILL IN HERE *) Admitted.
+  intros. apply E_Seq2; assumption.
+Qed.
 (** [] *)
 
 (** **** Exercise: 3 stars, advanced, optional (while_break_true) *)
@@ -2027,8 +2209,13 @@ Theorem while_break_true : forall b c st st',
   beval st' b = true ->
   exists st'', st'' =[ c ]=> st' / SBreak.
 Proof.
-(* FILL IN HERE *) Admitted.
-(** [] *)
+  intros. remember <{while b do c end}> as w eqn:Heqw.
+	induction H; try discriminate Heqw; injection Heqw as Heq1 Heq2; subst.
+	- apply IHceval2. reflexivity. assumption.
+	- rewrite H in H0. discriminate.
+	- exists st. assumption.
+Qed.
+(** [] *) 
 
 (** **** Exercise: 4 stars, advanced, optional (ceval_deterministic) *)
 Theorem ceval_deterministic: forall (c:com) st st1 st2 s1 s2,
